esqueleto

Conjunto.dfy
@@ -1,3 +1,36 @@
 class {:autocontracts} Conjunto{
-    
+    //implementacao
+    var arr: array<int>
+    //tamanho do conjunto
+    var tamanho: nat
+    //abstracao
+    ghost var Conteudo: set<int>
+    ghost var ConteudoSeq: seq<int>
+
+    //wip
+    predicate Valid(){
+        arr.Length > 0 &&
+        0 <= tamanho <=arr.Length &&
+        forall i, j :: 0 <= i < tamanho && 0 <= j < tamanho && i != j ==> arr[i] != arr[j] &&
+        Conteudo == 
+
+    }
+
+    constructor()
+
+    method Add() returns (b : bool)
+
+    method Remove() returns (b: bool)
+
+    method contains(i: int) returns (b: bool)
+
+    method Size() returns (s: int)
+
+    method isEmpty() returns (b: bool)
+
+    method Union(set2: Conjunto) returns (c: Conjunto)
+
+    method Intersec(set2: Conjunto) returns (c: Conjunto)
+
+    method Minus(sec2: Conjunto) returns (c: Conjunto)
 }
